protobuf-shim/proofs/fstar/extraction/test.sh
@@ -1,0 +1,32 @@
+
+    # Prints a path if and only if it exists. Takes one argument: the
+    # path.
+    function print_if_exists() {
+        if [ -d "$1" ]; then
+            echo "$1"
+        fi
+    }
+    # Asks Cargo all the dependencies for the current crate or workspace,
+    # and extract all "root" directories for each. Takes zero argument.
+    function dependencies() {
+        cargo metadata --format-version 1 |
+            jq -r '.packages | .[] | .manifest_path | split("/") | .[:-1] | join("/")'
+    }
+    # Find hax libraries *around* a given path. Takes one argument: the
+    # path.
+    function find_hax_libraries_at_path() {
+        path="$1"
+        # if there is a `proofs/fstar/extraction` subfolder, then that's a
+        # F* library
+        print_if_exists "$path/proofs/fstar/extraction"
+        # Maybe the `proof-libs` folder of hax is around?
+        MAYBE_PROOF_LIBS=$(realpath -q "$path/../proof-libs/fstar")
+        if [ $? -eq 0 ]; then
+            print_if_exists "$MAYBE_PROOF_LIBS/core"
+            print_if_exists "$MAYBE_PROOF_LIBS/rust_primitives"
+        fi
+    }
+    { while IFS= read path; do
+          find_hax_libraries_at_path "$path"
+      done < <(dependencies)
+    } | sort -u
